Fix errors due to notation change and flip substitution and weakening arguments

IMLTT/typed/JudgmentsAndRules.lean
@@ -44,7 +44,7 @@ mutual
     -- structural rules
     -- make sure variables of A refer to to same variables of Γ as before with lifting
     | var : IsType Γ A
-            → HasType (Γ ⬝ A) (.var 0) (weaken A (.shift .id))
+            → HasType (Γ ⬝ A) (.var 0) (weaken (.shift .id) A)
     -- | weak : HasType Γ (.var i) A → IsType Γ B
     --          → HasType (Γ ⬝ B) (.var (.succ i)) (weaken A (.shift .id))
     -- intro rules
@@ -77,13 +77,13 @@ mutual
                 → HasType Γ (.app f a) (substitute_zero B a)
     | sigma_elim : HasType Γ p (.sigma A B) → IsType (Γ ⬝ (.sigma A B)) C
                    → HasType (Γ ⬝ A ⬝ B) c
-                     (substitute C ((.weak (.shift (.shift .id))), .pairSigma (.var 1) (.var 0)))
+                     (substitute ((.weak (.shift (.shift .id))), .pairSigma (.var 1) (.var 0)) C)
                    → HasType Γ (.indSigma A B C c p) (substitute_zero C p)
-    | iden_elim : IsType (((Γ ⬝ A) ⬝ (weaken A (.shift .id)))
-                    ⬝ ( .iden (weaken A (.shift (.shift .id))) (.var 1) (.var 0))) B
-                  → HasType Γ b (substitute B ( .weak .id, a, a, .refl A a))
+    | iden_elim : IsType (((Γ ⬝ A) ⬝ (weaken (.shift .id) A))
+                    ⬝ (.iden (weaken (.shift (.shift .id)) A) (.var 1) (.var 0))) B
+                  → HasType Γ b (substitute ( .weak .id, a, a, .refl A a) B)
                   → HasType Γ p (.iden A a a')
-                  → HasType Γ (.j A B b a a' p) (substitute B (.weak .id, a, a', p))
+                  → HasType Γ (.j A B b a a' p) (substitute (.weak .id, a, a', p) B)
     -- conversion
     | ty_conv : HasType Γ a A → IsEqualType Γ A B
                 → HasType Γ a B
@@ -110,7 +110,7 @@ mutual
   @[aesop unsafe [constructors]]
   inductive IsEqualTerm : Ctx n → Tm n → Tm n → Tm n → Prop where
     | var_eq : IsType Γ A
-                → IsEqualTerm (Γ ⬝ A) (.var 0) (.var 0) (weaken A (.shift .id))
+                → IsEqualTerm (Γ ⬝ A) (.var 0) (.var 0) (weaken (.shift .id) A)
     -- computation rules
     | unit_comp : IsType (Γ ⬝ 𝟙) A → HasType Γ a (substitute_zero A .tt)
                   → IsEqualTerm Γ (.indUnit A .tt a) a (substitute_zero A .tt)
@@ -119,18 +119,18 @@ mutual
     | sigma_comp : HasType Γ a A → HasType Γ b (substitute_zero B a)
                    → IsType (Γ ⬝ (.sigma A B)) C
                    → HasType (Γ ⬝ A ⬝ B) c (
-                       substitute C ((.weak (.shift (.shift .id))), .pairSigma (.var 1) (.var 0))
+                       substitute ((.weak (.shift (.shift .id))), .pairSigma (.var 1) (.var 0)) C
                      )
                    → IsEqualTerm Γ (.indSigma A B C c (.pairSigma a b))
-                     (substitute c (.weak .id, a, b))
+                     (substitute (.weak .id, a, b) c)
                      (substitute_zero C (.pairSigma a b))
-    | iden_comp : IsType (((Γ ⬝ A) ⬝ (weaken A (.shift .id)))
-                    ⬝ ( .iden (weaken A (.shift (.shift .id))) (.var 1) (.var 0))) B
+    | iden_comp : IsType (((Γ ⬝ A) ⬝ (weaken (.shift .id) A))
+                    ⬝ (.iden (weaken (.shift (.shift .id)) A) (.var 1) (.var 0))) B
                   → HasType Γ b
-                    (substitute B (.weak .id, a, a, (.refl A a)))
+                    (substitute (.weak .id, a, a, (.refl A a)) B)
                   → HasType Γ a A
                   → IsEqualTerm Γ (.j A B b a a (.refl A a)) b
-                    (substitute B (.weak .id, a, a, (.refl A a)))
+                    (substitute (.weak .id, a, a, (.refl A a)) B)
     -- congruence rules (introduction and elimination)
     | unit_intro_eq : IsCtx Γ
                       → IsEqualTerm Γ .tt .tt 𝟙
@@ -149,21 +149,21 @@ mutual
                       → IsEqualTerm Γ p p' (.sigma A B)
                       → IsEqualType (Γ ⬝ (.sigma A B)) C C'
                       → IsEqualTerm (Γ ⬝ A ⬝ B) c c' (
-                          substitute C ((.weak (.shift (.shift .id))),
-                                          .pairSigma (.var 1) (.var 0))
+                          substitute ((.weak (.shift (.shift .id))),
+                                          .pairSigma (.var 1) (.var 0)) C
                         )
                       → IsEqualTerm Γ (.indSigma A B C c p) (.indSigma A' B' C' c' p')
                         (substitute_zero C p)
     | iden_intro_eq : IsEqualType Γ A A' → IsEqualTerm Γ a a' A
                       → IsEqualTerm Γ (.refl A a) (.refl A' a') (.iden A a a)
-    | iden_elim_eq : IsEqualType (((Γ ⬝ A) ⬝ (weaken A (.shift .id))) ⬝ (
-                          .iden (weaken A (.shift (.shift .id))) (.var 1) (.var 0)
+    | iden_elim_eq : IsEqualType (((Γ ⬝ A) ⬝ (weaken (.shift .id) A)) ⬝ (
+                          .iden (weaken (.shift (.shift .id)) A) (.var 1) (.var 0)
                         )) B B'
-                     → IsEqualTerm Γ b b' (substitute B (.weak .id, a₁, a₁, .refl A a₁))
+                     → IsEqualTerm Γ b b' (substitute (.weak .id, a₁, a₁, .refl A a₁) B)
                      → IsEqualType Γ (.iden A a₁ a₃) (.iden A' a₂ a₄)
                      → IsEqualTerm Γ p p' (.iden A a₁ a₃)
                      → IsEqualTerm Γ (.j A B b a₁ a₃ p) (.j A' B' b' a₂ a₄ p')
-                       (substitute B (.weak .id, a₁, a₃, p))
+                       (substitute (.weak .id, a₁, a₃, p) B)
     | univ_unit_eq : IsCtx Γ
                      → IsEqualTerm Γ 𝟙 𝟙 𝒰
     | univ_empty_eq : IsCtx Γ
