IMLTT/untyped/Weakening.lean
@@ -25,41 +25,41 @@ def lift_weak_n (i : Nat) (ρ : Weak m n) : Weak (m + i) (n + i) :=
   | 0 => ρ
   | i' + 1 => .lift (lift_weak_n i' ρ)
 
-def weaken_var (x : Fin n) (ρ : Weak m n) : Fin m :=
+def weaken_var (ρ : Weak m n) (x : Fin n) : Fin m :=
   match ρ with
   | .id => x
-  | .shift ρ => .succ (weaken_var x ρ)
+  | .shift ρ => .succ (weaken_var ρ x)
   | .lift ρ =>
     match x with
     | ⟨0, _⟩ => 0
-    | ⟨x' + 1, h⟩ => .succ (weaken_var (Fin.mk x' (Nat.lt_of_succ_lt_succ h)) ρ)
+    | ⟨x' + 1, h⟩ => .succ (weaken_var ρ (Fin.mk x' (Nat.lt_of_succ_lt_succ h)))
 
-def weaken (t : Tm n) (ρ : Weak m n) : Tm m :=
+def weaken (ρ : Weak m n) (t : Tm n) : Tm m :=
   match t with
   | .unit => .unit
   | .empty => .empty
-  | .pi A B => .pi (weaken A ρ) (weaken B (lift_weak_n 1 ρ))
-  | .sigma A B => .sigma (weaken A ρ) (weaken B (lift_weak_n 1 ρ))
-  | .iden A a a' => .iden (weaken A ρ) (weaken a ρ) (weaken a' ρ)
+  | .pi A B => .pi (weaken ρ A) (weaken (lift_weak_n 1 ρ) B)
+  | .sigma A B => .sigma (weaken ρ A) (weaken (lift_weak_n 1 ρ) B)
+  | .iden A a a' => .iden (weaken ρ A) (weaken ρ a) (weaken ρ a')
   | .univ => .univ
-  | .var i => weaken_var i ρ
+  | .var i => weaken_var ρ i
   | .tt => .tt
-  | .indUnit A b a => .indUnit (weaken A (lift_weak_n 1 ρ)) (weaken b ρ) (weaken a ρ)
-  | .indEmpty A b => .indEmpty (weaken A (lift_weak_n 1 ρ)) (weaken b ρ)
-  | .lam A b => .lam (weaken A ρ) (weaken b (lift_weak_n 1 ρ))
-  | .app f a => .app (weaken f ρ) (weaken a ρ)
-  | .pairSigma a b => .pairSigma (weaken a ρ) (weaken b ρ)
-  | .indSigma A B C c p => .indSigma (weaken A ρ) (weaken B (lift_weak_n 1 ρ)) 
-                            (weaken C (lift_weak_n 1 ρ)) (weaken c (lift_weak_n 2 ρ)) (weaken p ρ)
-  | .refl A a => .refl (weaken A ρ) (weaken a ρ)
-  | .j A B b a a' p => .j (weaken A ρ) (weaken B (lift_weak_n 3 ρ)) (weaken b ρ)
-                        (weaken a ρ) (weaken a' ρ) (weaken p ρ)
+  | .indUnit A b a => .indUnit (weaken (lift_weak_n 1 ρ) A) (weaken ρ b) (weaken ρ a)
+  | .indEmpty A b => .indEmpty (weaken (lift_weak_n 1 ρ) A) (weaken ρ b)
+  | .lam A b => .lam (weaken ρ A) (weaken (lift_weak_n 1 ρ) b)
+  | .app f a => .app (weaken ρ f) (weaken ρ a)
+  | .pairSigma a b => .pairSigma (weaken ρ a) (weaken ρ b)
+  | .indSigma A B C c p => .indSigma (weaken ρ A) (weaken (lift_weak_n 1 ρ) B)
+                            (weaken (lift_weak_n 1 ρ) C) (weaken (lift_weak_n 2 ρ) c) (weaken ρ p)
+  | .refl A a => .refl (weaken ρ A) (weaken ρ a)
+  | .j A B b a a' p => .j (weaken ρ A) (weaken (lift_weak_n 3 ρ) B) (weaken ρ b)
+                        (weaken ρ a) (weaken ρ a') (weaken ρ p)
 
 def shift_tm : Tm n → Tm (n + 1)
-  | t => weaken t (.shift .id)
+  | t => weaken (.shift .id) t
 
 notation:max "id_" => Weak.id
 prefix:97 "↑" => Weak.shift -- TODO: change 'associativity' to prevent having to use parenthesis?
 prefix:97 "⇑" => Weak.lift
 infixl:96 "∘" => comp_weaken
-notation:95 A "⌊" ρ "⌋" => weaken A ρ
+notation:95 A "⌊" ρ "⌋" => weaken ρ A
