IMLTT/typed/proofs/Recursor.lean
@@ -1,6 +1,7 @@
 import IMLTT.untyped.AbstractSyntax
 import IMLTT.untyped.Weakening
 import IMLTT.untyped.Substitution
+
 import IMLTT.typed.JudgmentsAndRules
 
 set_option pp.proofs true
@@ -14,12 +15,12 @@ theorem judgment_recursor :
   (IsCtxEmpty : motive_1 ε IsCtx.empty)
   → (IsCtxExtend : ∀ {x : Nat} {Γ : Ctx x} {A : Tm x} (a : Γ ctx) (a_1 : Γ ⊢ A type),
     motive_1 Γ a → motive_2 Γ A a_1 → motive_1 (Γ ⬝ A) (IsCtx.extend a a_1))
-  → (IsTypeUnitForm : ∀ {n : Nat} {Γ : Ctx n} (a : Γ ctx), 
+  → (IsTypeUnitForm : ∀ {n : Nat} {Γ : Ctx n} (a : Γ ctx),
     motive_1 Γ a → motive_2 Γ 𝟙 (IsType.unit_form a))
-  → (IsTypeEmptyForm : ∀ {n : Nat} {Γ : Ctx n} (a : Γ ctx), 
+  → (IsTypeEmptyForm : ∀ {n : Nat} {Γ : Ctx n} (a : Γ ctx),
     motive_1 Γ a → motive_2 Γ 𝟘 (IsType.empty_form a))
   → (IsTypePiForm : ∀ {n : Nat} {Γ : Ctx n} {A : Tm n} {B : Tm (n + 1)}
-    (a : Γ ⊢ A type) (a_1 : (Γ ⬝ A) ⊢ B type), 
+    (a : Γ ⊢ A type) (a_1 : (Γ ⬝ A) ⊢ B type),
     motive_2 Γ A a → motive_2 (Γ ⬝ A) B a_1 → motive_2 Γ (.pi A B) (IsType.pi_form a a_1))
   → (IsTypeSigmaForm : ∀ {n : Nat} {Γ : Ctx n} {A : Tm n} {B : Tm (n + 1)} 
     (a : Γ ⊢ A type) (a_1 : (Γ ⬝ A) ⊢ B type),
@@ -29,11 +30,11 @@ theorem judgment_recursor :
     motive_3 Γ a A a_1 → motive_3 Γ a' A a_2 
     → motive_2 Γ (.iden A a a') (IsType.iden_form a_1 a_2))
   → (IsTypeUnivForm : ∀ {n : Nat} {Γ : Ctx n}
-    (a : Γ ctx), motive_1 Γ a → motive_2 Γ U (IsType.univ_form a))
-  → (IsTypeUnivElim : ∀ {n : Nat} {Γ : Ctx n} {A : Tm n} (a : Γ ⊢ A ∶ U),
-    motive_3 Γ A U a → motive_2 Γ A (IsType.univ_elim a))
+    (a : Γ ctx), motive_1 Γ a → motive_2 Γ 𝒰 (IsType.univ_form a))
+  → (IsTypeUnivElim : ∀ {n : Nat} {Γ : Ctx n} {A : Tm n} (a : Γ ⊢ A ∶ 𝒰),
+    motive_3 Γ A 𝒰 a → motive_2 Γ A (IsType.univ_elim a))
   → (HasTypeVar : ∀ {x : Nat} {Γ : Ctx x} {A : Tm x} 
-    (a : Γ ⊢ A type), motive_2 Γ A a → motive_3 (Γ ⬝ A) v(0) (weaken A (.shift .id)) (HasType.var a))
+    (a : Γ ⊢ A type), motive_2 Γ A a → motive_3 (Γ ⬝ A) v(0) (weaken (.shift .id) A) (HasType.var a))
   → (HasTypeUnitIntro : ∀ {n : Nat} {Γ : Ctx n}
     (a : Γ ctx), motive_1 Γ a → motive_3 Γ ⋆ 𝟙 (HasType.unit_intro a))
   → (HasTypePiIntro : ∀ {n : Nat} {Γ : Ctx n} {A : Tm n} {b B : Tm (n + 1)} 
@@ -47,19 +48,19 @@ theorem judgment_recursor :
     motive_3 Γ a A a_2
     → motive_3 Γ (.refl A a) (.iden A a a) (HasType.iden_intro a_2))
   → (HasTypeUnivUnit : ∀ {n : Nat} {Γ : Ctx n} 
-    (a : Γ ctx), motive_1 Γ a → motive_3 Γ 𝟙 U (HasType.univ_unit a))
+    (a : Γ ctx), motive_1 Γ a → motive_3 Γ 𝟙 𝒰 (HasType.univ_unit a))
   → (HasTypeUnivEmpty : ∀ {n : Nat} {Γ : Ctx n} 
-    (a : Γ ctx), motive_1 Γ a → motive_3 Γ 𝟘 U (HasType.univ_empty a))
+    (a : Γ ctx), motive_1 Γ a → motive_3 Γ 𝟘 𝒰 (HasType.univ_empty a))
   → (HasTypeUnivPi : ∀ {n : Nat} {Γ : Ctx n} {A : Tm n} {B : Tm (n + 1)} 
-    (a : Γ ⊢ A ∶ U) (a_1 : (Γ ⬝ A) ⊢ B ∶ U),
-    motive_3 Γ A U a → motive_3 (Γ ⬝ A) B U a_1 → motive_3 Γ (.pi A B) U (HasType.univ_pi a a_1))
+    (a : Γ ⊢ A ∶ 𝒰) (a_1 : (Γ ⬝ A) ⊢ B ∶ 𝒰),
+    motive_3 Γ A 𝒰 a → motive_3 (Γ ⬝ A) B 𝒰 a_1 → motive_3 Γ (.pi A B) 𝒰 (HasType.univ_pi a a_1))
   → (HasTypeUnivSigma : ∀ {n : Nat} {Γ : Ctx n} {A : Tm n} {B : Tm (n + 1)} 
-    (a : Γ ⊢ A ∶ U) (a_1 : (Γ ⬝ A) ⊢ B ∶ U),
-    motive_3 Γ A U a → motive_3 (Γ ⬝ A) B U a_1 → motive_3 Γ (.sigma A B) U (HasType.univ_sigma a a_1))
+    (a : Γ ⊢ A ∶ 𝒰) (a_1 : (Γ ⬝ A) ⊢ B ∶ 𝒰),
+    motive_3 Γ A 𝒰 a → motive_3 (Γ ⬝ A) B 𝒰 a_1 → motive_3 Γ (.sigma A B) 𝒰 (HasType.univ_sigma a a_1))
   → (HasTypeUnivIden : ∀ {n : Nat} {Γ : Ctx n} {A a a' : Tm n} 
-    (a_1 : Γ ⊢ A ∶ U) (a_2 : Γ ⊢ a ∶ A) (a_3 : Γ ⊢ a' ∶ A),
-    motive_3 Γ A U a_1 → motive_3 Γ a A a_2 → motive_3 Γ a' A a_3 
-    → motive_3 Γ (.iden A a a') U (HasType.univ_iden a_1 a_2 a_3))
+    (a_1 : Γ ⊢ A ∶ 𝒰) (a_2 : Γ ⊢ a ∶ A) (a_3 : Γ ⊢ a' ∶ A),
+    motive_3 Γ A 𝒰 a_1 → motive_3 Γ a A a_2 → motive_3 Γ a' A a_3 
+    → motive_3 Γ (.iden A a a') 𝒰 (HasType.univ_iden a_1 a_2 a_3))
   → (HasTypeUnitElim : ∀ {n : Nat} {Γ : Ctx n} {A : Tm (n + 1)} {a b : Tm n} 
     (a_1 : (Γ ⬝ 𝟙) ⊢ A type) (a_2 : Γ ⊢ a ∶ substitute_zero A ⋆) (a_3 : Γ ⊢ b ∶ 𝟙),
     motive_2 (Γ ⬝ 𝟙) A a_1 → motive_3 Γ a (substitute_zero A ⋆) a_2 → motive_3 Γ b 𝟙 a_3 
@@ -75,21 +76,21 @@ theorem judgment_recursor :
   → (HasTypeSigmaElim : ∀ {n : Nat} {Γ : Ctx n} {A : Tm n} {B : Tm (n + 1)} {p : Tm n} 
     {C : Tm (n + 1)} {c : Tm (n + 1 + 1)}
     (a_1 : Γ ⊢ p ∶ (.sigma A B)) (a_2 : (Γ ⬝ (.sigma A B)) ⊢ C type)
-    (a_3 : (Γ ⬝ A ⬝ B) ⊢ c ∶ (substitute C (Subst.weak (.shift (.shift .id)), 
-      (.pairSigma v(1) v(0))))),
+    (a_3 : (Γ ⬝ A ⬝ B) ⊢ c ∶ (substitute (Subst.weak (.shift (.shift .id)), 
+      (.pairSigma v(1) v(0))) C)),
     motive_3 Γ p (.sigma A B) a_1 → motive_2 (Γ ⬝ (.sigma A B)) C a_2
     → motive_3 (Γ ⬝ A ⬝ B) c
-      (substitute C (Subst.weak (.shift (.shift .id)), (.pairSigma v(1) v(0)))) a_3
+      (substitute (Subst.weak (.shift (.shift .id)), (.pairSigma v(1) v(0))) C) a_3
     → motive_3 Γ (.indSigma A B C c p) (substitute_zero C p) (HasType.sigma_elim a_1 a_2 a_3) )
   → (HasTypeIdenElim : ∀ {n : Nat} {Γ : Ctx n} {A : Tm n} {B : Tm (n + 1 + 1 + 1)} {b : Tm n} 
     {a a' p : Tm n}
-    (a_1 : (Γ ⬝ A ⬝ weaken A Weak.id.shift ⬝ (weaken A Weak.id.shift.shift).iden v(1) v(0)) ⊢ B type)
-    (a_2 : Γ ⊢ b ∶ substitute B (Subst.weak .id, a, a, .refl A a))
+    (a_1 : (Γ ⬝ A ⬝ (weaken Weak.id.shift A) ⬝ (weaken Weak.id.shift.shift A).iden v(1) v(0)) ⊢ B type)
+    (a_2 : Γ ⊢ b ∶ substitute (Subst.weak .id, a, a, .refl A a) B)
     (a_4 : Γ ⊢ p ∶ A.iden a a'),
-    motive_2 (Γ ⬝ A ⬝ weaken A Weak.id.shift ⬝ (weaken A Weak.id.shift.shift).iden v(1) v(0)) B a_1 
-    → motive_3 Γ b (substitute B (Subst.weak .id, a, a, .refl A a)) a_2
+    motive_2 (Γ ⬝ A ⬝ weaken Weak.id.shift A ⬝ (weaken Weak.id.shift.shift A).iden v(1) v(0)) B a_1 
+    → motive_3 Γ b (substitute (Subst.weak .id, a, a, .refl A a) B) a_2
     → motive_3 Γ p (A.iden a a') a_4 
-    → motive_3 Γ (A.j B b a a' p) (substitute B (Subst.weak Weak.id, a, a', p)) 
+    → motive_3 Γ (A.j B b a a' p) (substitute (Subst.weak Weak.id, a, a', p) B) 
       (HasType.iden_elim a_1 a_2 a_4))
   → (HasTypeTyConv : ∀ {n : Nat} {Γ : Ctx n} {a A B : Tm n}
     (a_1 : Γ ⊢ a ∶ A) (a_2 : Γ ⊢ A ≡ B type), 
@@ -112,12 +113,12 @@ theorem judgment_recursor :
      motive_4 Γ A A' ae → motive_5 Γ a₁ a₂ A a → motive_5 Γ a₃ a₄ A' a_1
     → motive_4 Γ (A.iden a₁ a₃) (A'.iden a₂ a₄) (IsEqualType.iden_form_eq ae a a_1))
   → (IsEqualTypeUnivFormEq : ∀ {n : Nat} {Γ : Ctx n} 
-    (a : Γ ctx), motive_1 Γ a → motive_4 Γ U U (IsEqualType.univ_form_eq a))
+    (a : Γ ctx), motive_1 Γ a → motive_4 Γ 𝒰 𝒰 (IsEqualType.univ_form_eq a))
   → (IsEqualTypeUnivElimEq : ∀ {n : Nat} {Γ : Ctx n} {A A' : Tm n} 
-    (a : Γ ⊢ A ≡ A' ∶ U), motive_5 Γ A A' U a → motive_4 Γ A A' (IsEqualType.univ_elim_eq a))
+    (a : Γ ⊢ A ≡ A' ∶ 𝒰), motive_5 Γ A A' 𝒰 a → motive_4 Γ A A' (IsEqualType.univ_elim_eq a))
   → (IsEqualTermVarEq : ∀ {x : Nat} {Γ : Ctx x} {A : Tm x} 
     (a : Γ ⊢ A type), motive_2 Γ A a 
-    → motive_5 (Γ ⬝ A) v(0) v(0) (weaken A Weak.id.shift) (IsEqualTerm.var_eq a))
+    → motive_5 (Γ ⬝ A) v(0) v(0) (weaken Weak.id.shift A) (IsEqualTerm.var_eq a))
   → (IsEqualTermUnitComp : ∀ {n : Nat} {Γ : Ctx n} {A : Tm (n + 1)} {a : Tm n} 
     (a_1 : (Γ ⬝ 𝟙) ⊢ A type) (a_2 : Γ ⊢ a ∶ substitute_zero A ⋆),
     motive_2 (Γ ⬝ 𝟙) A a_1 → motive_3 Γ a (substitute_zero A ⋆) a_2 
@@ -129,24 +130,21 @@ theorem judgment_recursor :
   → (IsEqualTermSigmaComp : ∀ {n : Nat} {Γ : Ctx n} {a A b : Tm n} {B C : Tm (n + 1)} 
     {c : Tm (n + 1 + 1)} (a_1 : Γ ⊢ a ∶ A)
     (a_2 : Γ ⊢ b ∶ substitute_zero B a) (a_3 : (Γ ⬝ A.sigma B) ⊢ C type)
-    (a_4 : (Γ ⬝ A ⬝ B) ⊢ c ∶ substitute C (Subst.weak Weak.id.shift.shift, v(1).pairSigma v(0))),
+    (a_4 : (Γ ⬝ A ⬝ B) ⊢ c ∶ substitute (Subst.weak Weak.id.shift.shift, v(1).pairSigma v(0)) C),
     motive_3 Γ a A a_1 → motive_3 Γ b (substitute_zero B a) a_2 → motive_2 (Γ ⬝ A.sigma B) C a_3 
-    → motive_3 (Γ ⬝ A ⬝ B) c (substitute C (Subst.weak Weak.id.shift.shift, v(1).pairSigma v(0))) a_4 
-    → motive_5 Γ (A.indSigma B C c (a.pairSigma b)) (substitute c (Subst.weak Weak.id, a, b))
+    → motive_3 (Γ ⬝ A ⬝ B) c (substitute (Subst.weak Weak.id.shift.shift, v(1).pairSigma v(0)) C) a_4 
+    → motive_5 Γ (A.indSigma B C c (a.pairSigma b)) (substitute (Subst.weak Weak.id, a, b) c)
       (substitute_zero C (a.pairSigma b)) (IsEqualTerm.sigma_comp a_1 a_2 a_3 a_4))
   → (IsEqualTermIdenComp : ∀ {n : Nat} {Γ : Ctx n} {A : Tm n} {B : Tm (n + 1 + 1 + 1)} 
     {b : Tm n} {a : Tm n}
-    (a_1 : (Γ ⬝ A ⬝ weaken A Weak.id.shift ⬝ (weaken A Weak.id.shift.shift).iden v(1) v(0)) ⊢ B type)
-    (a_2 : Γ ⊢ b ∶ substitute B (Subst.weak Weak.id, a, a, .refl A a))
+    (a_1 : (Γ ⬝ A ⬝ (weaken Weak.id.shift A) ⬝ (weaken Weak.id.shift.shift A).iden v(1) v(0)) ⊢ B type)
+    (a_2 : Γ ⊢ b ∶ (substitute (Subst.weak Weak.id, a, a, .refl A a) B))
     (a_3 : Γ ⊢ a ∶ A),
-    motive_2 (Γ ⬝ A ⬝ weaken A Weak.id.shift ⬝ (weaken A Weak.id.shift.shift).iden v(1) v(0)) B a_1 
-  -- → HasType Γ b
-  --   (substitute B (.weak .id, a, a, (.refl A a)))
-    → motive_3 Γ b
-      (substitute B (Subst.weak Weak.id, a, a, .refl A a)) a_2 
-    → motive_3 Γ a A a_3 
+    motive_2 (Γ ⬝ A ⬝ (weaken Weak.id.shift A) ⬝ (weaken Weak.id.shift.shift A).iden v(1) v(0)) B a_1 
+    → motive_3 Γ b (substitute (Subst.weak Weak.id, a, a, .refl A a) B) a_2
+    → motive_3 Γ a A a_3
     → motive_5 Γ (A.j B b a a (A.refl a)) b
-      (substitute B (Subst.weak Weak.id, a, a, A.refl a)) (IsEqualTerm.iden_comp a_1 a_2 a_3))
+      (substitute (Subst.weak Weak.id, a, a, A.refl a) B) (IsEqualTerm.iden_comp a_1 a_2 a_3))
   → (IsEqualTermUnitIntroEq : ∀ {n : Nat} {Γ : Ctx n} 
     (a : Γ ctx), motive_1 Γ a → motive_5 Γ ⋆ ⋆ 𝟙 (IsEqualTerm.unit_intro_eq a))
   → (IsEqualTermUnitElimEq : ∀ {n : Nat} {Γ : Ctx n} {A A' : Tm (n + 1)} {a a' b b' : Tm n} 
@@ -172,10 +170,10 @@ theorem judgment_recursor :
     {B' : Tm (n + 1)} {p p' : Tm n} {C C' : Tm (n + 1)} {c c' : Tm (n + 1 + 1)} 
     (a : Γ ⊢ A.sigma B ≡ A'.sigma B' type) (a_1 : Γ ⊢ p ≡ p' ∶ A.sigma B)
     (a_2 : (Γ ⬝ A.sigma B) ⊢ C ≡ C' type)
-    (a_3 : (Γ ⬝ A ⬝ B) ⊢ c ≡ c' ∶ substitute C (Subst.weak Weak.id.shift.shift, v(1).pairSigma v(0))),
+    (a_3 : (Γ ⬝ A ⬝ B) ⊢ c ≡ c' ∶ substitute (Subst.weak Weak.id.shift.shift, v(1).pairSigma v(0)) C),
     motive_4 Γ (A.sigma B) (A'.sigma B') a → motive_5 Γ p p' (A.sigma B) a_1 
     → motive_4 (Γ ⬝ A.sigma B) C C' a_2 
-    → motive_5 (Γ ⬝ A ⬝ B) c c' (substitute C (Subst.weak Weak.id.shift.shift, v(1).pairSigma v(0))) a_3 
+    → motive_5 (Γ ⬝ A ⬝ B) c c' (substitute (Subst.weak Weak.id.shift.shift, v(1).pairSigma v(0)) C) a_3
     → motive_5 Γ (A.indSigma B C c p) (A'.indSigma B' C' c' p') (substitute_zero C p)
       (IsEqualTerm.sigma_elim_eq a a_1 a_2 a_3))
   → (IsEqualTermIdenIntroEq : ∀ {n : Nat} {Γ : Ctx n} {A A' a a' : Tm n} 
@@ -183,30 +181,30 @@ theorem judgment_recursor :
     → motive_5 Γ (A.refl a) (A'.refl a') (A.iden a a) (IsEqualTerm.iden_intro_eq a_1 a_2))
   → (IsEqualTermIdenElimEq : ∀ {n : Nat} {Γ : Ctx n} {A : Tm n} {B B' : Tm (n + 1 + 1 + 1)} 
     {b b' : Tm n} {a₁ a₃ A' a₂ a₄ p p' : Tm n}
-    (a : (Γ ⬝ A ⬝ weaken A Weak.id.shift ⬝ (weaken A Weak.id.shift.shift).iden v(1) v(0)) ⊢ B ≡ B' type)
-    (a_1 : Γ ⊢ b ≡ b' ∶ substitute B (Subst.weak Weak.id, a₁, a₁, .refl A a₁))
+    (a : (Γ ⬝ A ⬝ weaken Weak.id.shift A ⬝ (weaken Weak.id.shift.shift A).iden v(1) v(0)) ⊢ B ≡ B' type)
+    (a_1 : Γ ⊢ b ≡ b' ∶ substitute (Subst.weak Weak.id, a₁, a₁, .refl A a₁) B)
     (a_2 : Γ ⊢ A.iden a₁ a₃ ≡ A'.iden a₂ a₄ type) (a_3 : Γ ⊢ p ≡ p' ∶ A.iden a₁ a₃),
-    motive_4 (Γ ⬝ A ⬝ weaken A Weak.id.shift ⬝ (weaken A Weak.id.shift.shift).iden v(1) v(0)) B B' a 
+    motive_4 (Γ ⬝ A ⬝ weaken Weak.id.shift A ⬝ (weaken Weak.id.shift.shift A).iden v(1) v(0)) B B' a 
     → motive_5 Γ b b' 
-      (substitute B (Subst.weak Weak.id, a₁, a₁, .refl A a₁)) a_1
+      (substitute (Subst.weak Weak.id, a₁, a₁, .refl A a₁) B) a_1
     → motive_4 Γ (A.iden a₁ a₃) (A'.iden a₂ a₄) a_2 → motive_5 Γ p p' (A.iden a₁ a₃) a_3 
-    → motive_5 Γ (A.j B b a₁ a₃ p) (A'.j B' b' a₂ a₄ p') (substitute B (Subst.weak Weak.id, a₁, a₃, p))
+    → motive_5 Γ (A.j B b a₁ a₃ p) (A'.j B' b' a₂ a₄ p') (substitute (Subst.weak Weak.id, a₁, a₃, p) B)
       (IsEqualTerm.iden_elim_eq a a_1 a_2 a_3))
   → (IsEqualTermUnivUnitEq : ∀ {n : Nat} {Γ : Ctx n} 
-    (a : Γ ctx), motive_1 Γ a → motive_5 Γ 𝟙 𝟙 U (IsEqualTerm.univ_unit_eq a))
+    (a : Γ ctx), motive_1 Γ a → motive_5 Γ 𝟙 𝟙 𝒰 (IsEqualTerm.univ_unit_eq a))
   → (IsEqualTermUnivEmptyEq : ∀ {n : Nat} {Γ : Ctx n} 
-    (a : Γ ctx), motive_1 Γ a → motive_5 Γ 𝟘 𝟘 U (IsEqualTerm.univ_empty_eq a))
+    (a : Γ ctx), motive_1 Γ a → motive_5 Γ 𝟘 𝟘 𝒰 (IsEqualTerm.univ_empty_eq a))
   → (IsEqualTermUnivPiEq : ∀ {n : Nat} {Γ : Ctx n} {A A' : Tm n} {B B' : Tm (n + 1)} 
-    (a : Γ ⊢ A ≡ A' ∶ U) (a_1 : (Γ ⬝ A) ⊢ B ≡ B' ∶ U), motive_5 Γ A A' U a 
-    → motive_5 (Γ ⬝ A) B B' U a_1 → motive_5 Γ (A.pi B) (A'.pi B') U (IsEqualTerm.univ_pi_eq a a_1))
+    (a : Γ ⊢ A ≡ A' ∶ 𝒰) (a_1 : (Γ ⬝ A) ⊢ B ≡ B' ∶ 𝒰), motive_5 Γ A A' 𝒰 a 
+    → motive_5 (Γ ⬝ A) B B' 𝒰 a_1 → motive_5 Γ (A.pi B) (A'.pi B') 𝒰 (IsEqualTerm.univ_pi_eq a a_1))
   → (IsEqualTermUnivSigmaEq : ∀ {n : Nat} {Γ : Ctx n} {A A' : Tm n} {B B' : Tm (n + 1)} 
-    (a : Γ ⊢ A ≡ A' ∶ U) (a_1 : (Γ ⬝ A) ⊢ B ≡ B' ∶ U), motive_5 Γ A A' U a →
-    motive_5 (Γ ⬝ A) B B' U a_1 
-    → motive_5 Γ (A.sigma B) (A'.sigma B') U (IsEqualTerm.univ_sigma_eq a a_1))
+    (a : Γ ⊢ A ≡ A' ∶ 𝒰) (a_1 : (Γ ⬝ A) ⊢ B ≡ B' ∶ 𝒰), motive_5 Γ A A' 𝒰 a →
+    motive_5 (Γ ⬝ A) B B' 𝒰 a_1 
+    → motive_5 Γ (A.sigma B) (A'.sigma B') 𝒰 (IsEqualTerm.univ_sigma_eq a a_1))
   → (IsEqualTermUnivIdenEq : ∀ {n : Nat} {Γ : Ctx n} {A A' a₁ a₂ a₃ a₄ : Tm n} 
-    (a : Γ ⊢ A ≡ A' ∶ U) (a_1 : Γ ⊢ a₁ ≡ a₂ ∶ A) (a_2 : Γ ⊢ a₃ ≡ a₄ ∶ A), motive_5 Γ A A' U a 
+    (a : Γ ⊢ A ≡ A' ∶ 𝒰) (a_1 : Γ ⊢ a₁ ≡ a₂ ∶ A) (a_2 : Γ ⊢ a₃ ≡ a₄ ∶ A), motive_5 Γ A A' 𝒰 a 
     → motive_5 Γ a₁ a₂ A a_1 → motive_5 Γ a₃ a₄ A a_2 
-    → motive_5 Γ (A.iden a₁ a₃) (A'.iden a₂ a₄) U (IsEqualTerm.univ_iden_eq a a_1 a_2))
+    → motive_5 Γ (A.iden a₁ a₃) (A'.iden a₂ a₄) 𝒰 (IsEqualTerm.univ_iden_eq a a_1 a_2))
   → (IsEqualTermTyConvEq : ∀ {n : Nat} {Γ : Ctx n} {a b A B : Tm n} 
     (a_1 : Γ ⊢ a ≡ b ∶ A) (a_2 : Γ ⊢ A ≡ B type), motive_5 Γ a b A a_1 → motive_4 Γ A B a_2 
     → motive_5 Γ a b B (IsEqualTerm.ty_conv_eq a_1 a_2))
