IMLTT/typed/proofs/admissable/Weakening.lean
@@ -8,7 +8,7 @@ import IMLTT.typed.proofs.Recursor
 import IMLTT.typed.proofs.boundary.BoundaryIsCtx
 
 theorem og_weak : HasType Γ (.var i) A → IsType Γ B
-                  → HasType (Γ ⬝ B) (.var (.succ i)) (weaken A (.shift .id)) :=
+                  → HasType (Γ ⬝ B) (.var (.succ i)) (weaken (.shift .id) A) :=
   by
     intro hiA hB
     match hB with
@@ -16,32 +16,32 @@ theorem og_weak : HasType Γ (.var i) A → IsType Γ B
 
 theorem weakening :
   (∀ {n : Nat} {Γ : Ctx n}, Γ ctx → ∀ (B A : Tm n), Γ ⬝ A ctx → Γ ⊢ B type 
-    → Γ ⬝ B ⬝ weaken A Weak.id.shift ctx) ∧
+    → Γ ⬝ B ⬝ weaken Weak.id.shift A ctx) ∧
   (∀ {n : Nat} {Γ : Ctx n} {A : Tm n}, Γ ⊢ A type → ∀ (B : Tm n), Γ ⊢ B type 
-    → Γ ⬝ B ⊢ weaken A Weak.id.shift type) ∧
+    → Γ ⬝ B ⊢ weaken Weak.id.shift A type) ∧
   (∀ {n : Nat} {Γ : Ctx n} {A a : Tm n}, (Γ ⊢ a ∶ A) → ∀ (B : Tm n), Γ ⊢ B type 
-    → Γ ⬝ B ⊢ weaken a Weak.id.shift ∶ weaken A Weak.id.shift) ∧
+    → Γ ⬝ B ⊢ weaken Weak.id.shift a ∶ weaken Weak.id.shift A) ∧
   (∀ {n : Nat} {Γ : Ctx n} {A A' : Tm n}, Γ ⊢ A ≡ A' type → ∀ (B : Tm n), Γ ⊢ B type 
-    → Γ ⬝ B ⊢ weaken A Weak.id.shift ≡ weaken A' Weak.id.shift type) ∧
+    → Γ ⬝ B ⊢ weaken Weak.id.shift A ≡ weaken  Weak.id.shift A' type) ∧
   (∀ {n : Nat} {Γ : Ctx n} {A a a' : Tm n}, (Γ ⊢ a ≡ a' ∶ A) → ∀ (B : Tm n), Γ ⊢ B type 
-    → Γ ⬝ B ⊢ weaken a Weak.id.shift ≡ weaken a' Weak.id.shift ∶ weaken A Weak.id.shift) :=
+    → Γ ⬝ B ⊢ weaken Weak.id.shift a ≡ weaken Weak.id.shift a' ∶ weaken Weak.id.shift A) :=
   by
     apply judgment_recursor
       (motive_1 := fun Γ _hiC =>
         ∀B, ∀ A, Γ ⬝ A ctx → Γ ⊢ B type
-        → Γ ⬝ B ⬝ (weaken A (.shift .id)) ctx)
+        → Γ ⬝ B ⬝ (weaken (.shift .id) A) ctx)
       (motive_2 := fun Γ A _hA =>
         ∀B, Γ ⊢ B type
-        → Γ ⬝ B ⊢ (weaken A (.shift .id)) type)
+        → Γ ⬝ B ⊢ (weaken (.shift .id) A) type)
       (motive_3 := fun Γ a A haA =>
         ∀B, Γ ⊢ B type
-        → HasType (Γ ⬝ B) (weaken a (.shift .id)) (weaken A (.shift .id)))
+        → HasType (Γ ⬝ B) (weaken (.shift .id) a) (weaken (.shift .id) A))
       (motive_4 := fun Γ A A' _hAA =>
         ∀B, Γ ⊢ B type
-        → Γ ⬝ B ⊢ (weaken A (.shift .id)) ≡ (weaken A' (.shift .id)) type)
+        → Γ ⬝ B ⊢ (weaken (.shift .id) A) ≡ (weaken (.shift .id) A') type)
       (motive_5 := fun Γ a a' A _haaA =>
         ∀B, Γ ⊢ B type
-        → Γ ⬝ B ⊢ (weaken a (.shift .id)) ≡ (weaken a' (.shift .id)) ∶ (weaken A (.shift .id)))
+        → Γ ⬝ B ⊢ (weaken (.shift .id) a) ≡ (weaken (.shift .id) a') ∶ (weaken (.shift .id)) A)
     case IsCtxEmpty =>
       -- ⊢ ∀ (B A : Tm 0), ε ⬝ A ctx → ε ⊢ B type → ε ⬝ B ⬝ (A⌊↑id⌋) ctx
       intro B A hiA hB
@@ -53,7 +53,7 @@ theorem weakening :
     any_goals sorry
 
 theorem weakening_ctx : IsCtx (Γ ⬝ A) → IsType Γ B
-                        → IsCtx (Γ ⬝ B ⬝ (weaken A (.shift .id))) :=
+                        → IsCtx (Γ ⬝ B ⬝ (weaken (.shift .id) A)) :=
   by
     intro hiCA hB
     apply And.left weakening
@@ -62,7 +62,7 @@ theorem weakening_ctx : IsCtx (Γ ⬝ A) → IsType Γ B
     · apply hB
 
 theorem weakening_type : IsType Γ A → IsType Γ B
-                         → IsType (Γ ⬝ B) (weaken A (.shift .id)) :=
+                         → IsType (Γ ⬝ B) (weaken (.shift .id) A) :=
   by
     intro hA hB
     apply And.left (And.right weakening)
@@ -71,8 +71,8 @@ theorem weakening_type : IsType Γ A → IsType Γ B
 
 
 theorem weakening_term : HasType Γ a A → IsType Γ B
-                         → HasType (Γ ⬝ B) (weaken a (.shift .id)) 
-                           (weaken A (.shift .id)) :=
+                         → HasType (Γ ⬝ B) (weaken (.shift .id) a) 
+                           (weaken (.shift .id) A) :=
   by
     intro haA hB
     apply And.left (And.right (And.right weakening))
@@ -80,8 +80,8 @@ theorem weakening_term : HasType Γ a A → IsType Γ B
     · apply hB
 
 theorem weakening_type_eq : IsEqualType Γ A A' → IsType Γ B
-                            → IsEqualType (Γ ⬝ B) (weaken A (.shift .id)) 
-                              (weaken A' (.shift .id)) :=
+                            → IsEqualType (Γ ⬝ B) (weaken (.shift .id) A)
+                              (weaken (.shift .id) A') :=
   by
     intro hAA hB
     apply And.left (And.right (And.right (And.right weakening)))
@@ -89,9 +89,9 @@ theorem weakening_type_eq : IsEqualType Γ A A' → IsType Γ B
     · apply hB
 
 theorem weakening_term_eq : IsEqualTerm Γ a a' A → IsType Γ B
-                            → IsEqualTerm (Γ ⬝ B) (weaken a (.shift .id)) 
-                              (weaken a' (.shift .id))
-                              (weaken A (.shift .id)) :=
+                            → IsEqualTerm (Γ ⬝ B) (weaken (.shift .id) a)
+                              (weaken (.shift .id) a')
+                              (weaken (.shift .id) A) :=
   by
     intro haaA hB
     apply And.right (And.right (And.right (And.right weakening)))
